Experimenting new salloc

specs/lib/Spec.Lib.IntBuf.fsti
@@ -97,6 +97,34 @@ inline_for_extraction val salloc: #a:Type0 -> #b:Type0 -> #len:size_nat -> clen:
 					           modifies writes h0 h1 /\
 					           spec h0 r h1))
 
+
+// Experiment
+let salloc'_inv (h0:mem) (h1:mem) (#a:Type) (#b:Type0) (len:size_nat)  (buf:lbuffer a len) (init:a) (reads:list bufitem) (writes:list bufitem)
+  (spec:(h:mem -> b -> mem -> Type)) : Type =
+  lives h0 reads /\ lives h0 writes
+  /\ preserves_live h0 h1
+  /\ disjoint_list buf reads /\ disjoint_list buf writes
+  /\ as_lseq #a #len buf h1 == LSeq.create #a len init
+
+inline_for_extraction val salloc':
+  #h0:mem -> #a:Type0 -> #b:Type0 -> #len:size_nat ->
+  clen:size_t{v clen == len} ->
+  init:a ->
+  reads:list bufitem ->
+  writes:list bufitem ->
+  spec:(h0:mem -> r:b -> h1:mem -> Type) ->
+  impl:(buf:lbuffer a len -> Stack b
+    (requires (fun h -> salloc'_inv h0 h #a len buf init reads writes spec))
+	 (ensures (fun h0 r h1 -> salloc'_inv h0 h1 #a len buf init reads writes spec /\
+				              modifies (BufItem buf :: writes) h0 h1 /\
+						        spec h0 r h1))) ->
+  Stack b
+    (requires (fun h0 -> live_list h0 reads /\ live_list h0 writes /\ disjoints reads /\ disjoints writes))
+    (ensures (fun h0 r h1 -> preserves_live h0 h1 /\
+					           modifies writes h0 h1 /\
+					           spec h0 r h1))
+
+
 inline_for_extraction let op_Array_Assignment #a #len = upd #a #len
 inline_for_extraction let op_Array_Access #a #len = index #a #len
 
